CookLevin/Complexity/Lang.lean
@@ -7,6 +7,7 @@ import Complexity.Lang.ScanPast
 import Complexity.Lang.ScanLeft
 import Complexity.Lang.AppendGadget
 import Complexity.Lang.AcceptHalt
+import Complexity.Lang.FormatCheck
 import Complexity.Lang.Compile
 import Complexity.Lang.PolyTime
 
